definition des morphismes et unicite du morphisme

main.v
@@ -5,7 +5,7 @@ Set Implicit Arguments.
 Unset Strict Implicit.
 Unset Printing Implicit Defensive.
 
-(* on pourrait aussi faire { A : Type & A -> list nat}, comme def de signature *)
+(* Signatures could alternatively be defined as { A : Type & A -> list nat} *)
 Definition sig := list nat -> Type.
 
 Definition sig_LC : sig :=
@@ -14,7 +14,7 @@ Definition sig_LC : sig :=
            | _ => False
            end.
 
-(* Vec A B l, c'est une liste d'elements de A de meme taille que l *)
+(* Vec {A} B l is a B-list of the same size as l *)
 Inductive Vec {A : Type} (B : Type) : list A -> Type :=
     NilV : Vec B nil
   | ConsV : forall a lA, B -> Vec B lA -> Vec B (a :: lA).
@@ -23,7 +23,7 @@ Inductive Vec {A : Type} (B : Type) : list A -> Type :=
 
 Inductive Z (Sig : sig) : Type :=
   Var : nat -> Z Sig
-| Op : forall ar, Sig ar -> Vec (Z Sig) ar (* en gros, c'est Z^(length ar) *) -> Z Sig.
+| Op : forall ar, Sig ar -> Vec (Z Sig) ar (* this is Z^(length ar) *) -> Z Sig.
 
 
 Definition Vec_map {A B C : Type}(f : A -> B -> C) :=
@@ -38,10 +38,10 @@ Lemma vec_map_map {A B C D : Type}(f : A -> B -> C) (g : A -> C -> D) {l : list 
   induction v; cbn; congruence.
 Qed.
 
-Lemma vec_map_fun_ext {A B C : Type}(f g : A -> B -> C) {l : list A}
+Definition vec_map_fun_ext {A B C : Type}(f g : A -> B -> C) {l : list A}
       (v : Vec B l) (h : forall a b, f a b = g a b): Vec_map f v = Vec_map g v.
   induction v; cbn; congruence.
-Qed.
+Defined.
 
 
 
@@ -67,11 +67,11 @@ Record model (Sig : sig) :=
     substitution : (nat -> carrier) -> carrier -> carrier ;
     ops : forall (ar : list nat), Sig ar -> Vec carrier ar ->
                                              carrier;
-    (* fun ext pour la substitution *)
-    substitution_ext : forall f g x,  (forall n, f n = g n) -> 
+    (* fun ext for substitution *)
+    substitution_ext : forall f g ,  (forall n, f n = g n) -> forall x,
                                     substitution f x = substitution g x;
     variables_eq : forall x f, substitution f (variables x) = f x;
-    (* les operations sont des morphismes de module *)
+    (* operations are module morphisms *)
     ops_eq : forall (ar : list nat)
                     (o : Sig ar)
                     (v : Vec carrier ar)
@@ -85,6 +85,74 @@ Record model (Sig : sig) :=
                      
   }.
 
+Record model_mor {Sig : sig} (X : model Sig) (Y : model Sig) :=
+  { carrier_mor :> X -> Y ;
+    variables_mor : forall n, carrier_mor (variables X n) = variables Y n ;
+    substitution_mor : forall (f : nat -> X) (x : X), carrier_mor (substitution f x) =
+                                              substitution (fun n => carrier_mor (f n))
+                                                           (carrier_mor x) ;
+    ops_mor : forall (ar : list nat)(s : Sig ar)(v : Vec X ar), carrier_mor (ops s v) =
+                                                         ops s (Vec_map (fun _ => carrier_mor) v)
+  
+  }.
+
+(* Z is a model *)
+
+
+Fixpoint Z_subst_funext {Sig}(f g : nat -> Z Sig) (eq : forall n, f n = g n) x :
+  Z_subst f x = Z_subst g x.
+Proof.
+  destruct x.
+  - cbn; apply eq.
+  - cbn.
+    f_equal.
+    apply vec_map_fun_ext.
+    intros.
+    apply Z_subst_funext.
+    intro.
+    rewrite eq.
+    reflexivity.
+Qed.
+
+Fixpoint Z_ren_subst_eq {Sig} (f : nat -> nat) (x : Z Sig) :
+  Z_ren f x = Z_subst (fun n => Var Sig (f n)) x.
+Proof.
+  destruct x.
+  - reflexivity.
+  - cbn.
+    f_equal.
+    apply vec_map_fun_ext.
+    intros.
+    rewrite Z_ren_subst_eq.
+    cbn.
+    apply Z_subst_funext.
+    intro.
+    destruct a; [reflexivity|].
+    destruct (n <=? a); reflexivity.
+Qed.
+          
+
+
+Program Definition ZModel (Sig : sig) : model Sig :=
+  {|
+  carrier := Z Sig;
+  variables := Var Sig;
+  substitution := Z_subst;
+  ops := @Op Sig;
+  substitution_ext := Z_subst_funext
+  |}.
+Next Obligation.
+  cbn.
+  f_equal.
+  apply vec_map_fun_ext.
+  intros.
+  apply Z_subst_funext.
+  intro.
+  rewrite Z_ren_subst_eq.
+  reflexivity.
+Qed.
+
+(* the initial morphism *)
 
 Fixpoint ini_mor {Sig : sig} (m : model Sig )(x : Z Sig) : m :=
   match x with
@@ -92,7 +160,7 @@ Fixpoint ini_mor {Sig : sig} (m : model Sig )(x : Z Sig) : m :=
       | @Op _ ar op v   => ops op (Vec_map (fun _ => ini_mor m) v)
   end.
 
-(* le morphisme initial preserve le renommage *)
+(* the initial morphism preserves renaming *)
 Fixpoint mor_ren { Sig : sig}(m : model Sig)(f : nat -> nat) (x : Z Sig) :
   ini_mor m (Z_ren f x) = substitution (fun y => variables _ (f y)) (ini_mor m x).
   destruct x as [n|ar o v].
@@ -122,8 +190,8 @@ Fixpoint mor_ren { Sig : sig}(m : model Sig)(f : nat -> nat) (x : Z Sig) :
 Defined.
 
 
-(* le morphisme initial preserve la substitution *)
-Fixpoint mor_subst { Sig : sig}(m : model Sig)(f : nat -> Z Sig) (x : Z Sig) :
+(* the initial morphism preserves substitution *)
+Fixpoint mor_subst {Sig : sig}(m : model Sig)(f : nat -> Z Sig) (x : Z Sig) :
   ini_mor m (Z_subst f x) = substitution (fun y => ini_mor m (f y)) (ini_mor m x).
   destruct x as [n|ar o v].
   - cbn.
@@ -149,3 +217,26 @@ Fixpoint mor_subst { Sig : sig}(m : model Sig)(f : nat -> Z Sig) (x : Z Sig) :
         --  reflexivity.
         --  apply mor_ren.
 Defined.
+
+
+Program Definition initial_morphism {Sig : sig}(m : model Sig) : model_mor (ZModel Sig) m :=
+  {|
+  carrier_mor := ini_mor m;
+  |}.
+Next Obligation.
+  apply mor_subst.
+Qed.
+
+Fixpoint initial_morphism_unique {Sig : sig}(m : model Sig) (f : model_mor (ZModel Sig) m)
+     x : f x = initial_morphism m x. 
+Proof.
+  destruct x.
+  - apply variables_mor.
+  - etransitivity.
+    apply ops_mor.
+    cbn.
+    f_equal.
+    apply vec_map_fun_ext.
+    intros.
+    apply initial_morphism_unique.
+Qed.
